soundness proof for specialisation of expressions

Coq/Denotational.v
@@ -77,9 +77,7 @@ Fixpoint Acc_sem {A} (f : nat -> A -> A) (n : nat) (z : A) : A :=
 Lemma Acc_sem_ind A (P : A -> Prop) f n z : (forall i (x : A), P x -> P (f i x)) ->  
                                             P z -> P (Acc_sem f n z).
 Proof.
-  intros F Z. induction n. 
-  - simpl. auto.
-  - simpl. remember (Acc_sem f n z) as x. auto.
+  intros F Z. induction n; simpl;auto.
 Qed.
 
 (* Semantics of operations *)
@@ -121,14 +119,16 @@ Fixpoint lookupEnv (v : Var) (rho : Env) : option Val :=
 
 Reserved Notation "'E[|' e '|]'" (at level 9).
 
+Definition Fsem {A} (f : Env -> ExtEnv -> option A) (rho : Env) (erho : ExtEnv) 
+  := (fun m x => x >>= fun x' =>  f (x' :: rho) (adv_ext (Z.of_nat m) erho)).
+
 Fixpoint Esem (e : Exp) (rho : Env) (erho : ExtEnv) : option Val :=
     match e with
       | OpE op args => sequence (map (fun e => E[|e|] rho erho) args) >>= OpSem op
       | Obs l i => Some (erho l i)
       | VarE v => lookupEnv v rho
       | Acc f l z => let erho' := adv_ext (- Z.of_nat l) erho
-                     in Acc_sem (fun m x => x >>= fun x' => E[| f |] (x' :: rho) 
-                                              (adv_ext (Z.of_nat m) erho')) l (E[|z|] rho erho')
+                     in Acc_sem (Fsem E[|f|] rho erho') l (E[|z|] rho erho')
     end
       where "'E[|' e '|]'" := (Esem e ). 
 
