Coq/SyntacticCausality.v
@@ -69,12 +69,13 @@ Proof.
   - simpl; unfold ext_until in O. rewrite O. reflexivity. omega.
   - do 4 (eapply all_apply in H0;eauto).
     apply map_rewrite in H0. simpl. rewrite H0. reflexivity.
-  - generalize dependent vars. generalize dependent r2. generalize dependent r1. induction l; intros. 
+  - generalize dependent vars. generalize dependent r2. generalize dependent r1. 
+    induction l; intros. 
     + simpl. apply IHR2. assumption.
     + pose (adv_ext_step l (A:=Val)) as RE. simpl in *. do 2 rewrite RE.
       erewrite IHl. apply bind_equals. apply IHl. apply ext_until_adv. eapply ext_until_le. eauto.
       omega. intros. apply IHR1.  apply ext_until_adv. do 2 rewrite adv_ext_iter. apply ext_until_adv. 
-      eapply ext_until_le.  apply O. rewrite Zpos_P_of_succ_nat.
+      eapply ext_until_le.  apply O. rewrite Nat2Z.inj_succ.
       omega. constructor.
 Qed.
 
